theories/Eq/Shallow.v
@@ -64,7 +64,7 @@ Record observing {E R1 R2}
            (t1 : itree E R1) (t2 : itree E R2) : Prop :=
   observing_intros
   { observing_observe : eq_ (observe t1) (observe t2) }.
-#[global] Hint Constructors observing: core.
+#[global] Hint Constructors observing : itree.
 
 Section observing_relations.
 
@@ -78,21 +78,21 @@ Proof. intros ? ? []; cbv; auto. Qed.
 
 #[global]
 Instance observing_go : Proper (eq_ ==> observing eq_) (@go E R).
-Proof. cbv; auto. Qed.
+Proof. cbv; auto with itree. Qed.
 
 #[global]
 Instance monotonic_observing eq_' :
   subrelation eq_ eq_' ->
   subrelation (observing eq_) (observing eq_').
-Proof. intros ? ? ? []; cbv; eauto. Qed.
+Proof. intros ? ? ? []; cbv; eauto with itree. Qed.
 
 #[global]
 Instance Equivalence_observing :
   Equivalence eq_ -> Equivalence (observing eq_).
-Proof.
-  intros []; split; cbv; auto.
-  - intros ? ? []; auto.
-  - intros ? ? ? [] []; eauto.
+Proof with (auto with itree).
+  intros []; split; cbv...
+  - intros ? ? []; auto...
+  - intros ? ? ? [] []; eauto with itree.
 Qed.
 
 End observing_relations.
@@ -139,12 +139,12 @@ Proof. econstructor. reflexivity. Qed.
 Inductive going {E R1 R2} (r : itree E R1 -> itree E R2 -> Prop)
           (ot1 : itree' E R1) (ot2 : itree' E R2) : Prop :=
 | going_intros : r (go ot1) (go ot2) -> going r ot1 ot2.
-#[global] Hint Constructors going: core.
+#[global] Hint Constructors going : itree.
 
 Lemma observing_going {E R1 R2} (eq_ : itree' E R1 -> itree' E R2 -> Prop) ot1 ot2 :
   going (observing eq_) ot1 ot2 <-> eq_ ot1 ot2.
 Proof.
-  split; auto.
+  split; auto with itree.
   intros [[]]; auto.
 Qed.
 
@@ -161,15 +161,15 @@ Proof. intros ? ? []; auto. Qed.
 Instance monotonic_going eq_' :
   subrelation eq_ eq_' ->
   subrelation (going eq_) (going eq_').
-Proof. intros ? ? ? []; eauto. Qed.
+Proof. intros ? ? ? []; eauto with itree. Qed.
 
 #[global]
 Instance Equivalence_going :
   Equivalence eq_ -> Equivalence (going eq_).
 Proof.
-  intros []; constructor; cbv; eauto.
-  - intros ? ? []; auto.
-  - intros ? ? ? [] []; eauto.
+  intros []; constructor; cbv; eauto with itree.
+  - intros ? ? []; auto with itree.
+  - intros ? ? ? [] []; eauto with itree.
 Qed.
 
 End going_relations.
